theories/MSets/MSetList.v
@@ -790,20 +790,20 @@ Module MakeRaw (X: OrderedType) <: RawSets X.
    split; auto. transitivity s4; auto.
   Qed.
 
-  Lemma compare_spec_aux : forall s s', Cmp eq L.lt s s' (compare s s').
+  Lemma compare_spec_aux : forall s s', CompSpec eq L.lt s s' (compare s s').
   Proof.
   induction s as [|x s IH]; intros [|x' s']; simpl; intuition.
   elim_compare x x'; auto.
   Qed.
 
   Lemma compare_spec : forall s s', Ok s -> Ok s' ->
-   Cmp eq lt s s' (compare s s').
+   CompSpec eq lt s s' (compare s s').
   Proof.
   intros s s' Hs Hs'.
   generalize (compare_spec_aux s s').
   destruct (compare s s'); inversion_clear 1; auto.
-  apply Cmp_lt. exists s, s'; repeat split; auto using @ok.
-  apply Cmp_gt. exists s', s; repeat split; auto using @ok.
+  apply CompLt. exists s, s'; repeat split; auto using @ok.
+  apply CompGt. exists s', s; repeat split; auto using @ok.
   Qed.
 
 End MakeRaw.
